revising hash accumulator to use a counter and updating interfaces upstream

steel/Veritas.Steel.HashAccumulator.fst
@@ -1,23 +1,48 @@
 module Veritas.Steel.HashAccumulator
 module U8 = FStar.UInt8
 module U32 = FStar.UInt32
+module U64 = FStar.UInt64
+module Cast = FStar.Int.Cast
 module A = Steel.Array
 
 open Steel.Memory
 open Steel.Effect.Common
 open Steel.Effect
-open Steel.Reference
 module AT = Steel.Effect.Atomic
 module Blake = Hacl.Blake2b_32
 module Loops = Steel.Loops
-#push-options "--fuel 0 --ifuel 0"
+module R = Steel.Reference
+#push-options "--ide_id_info_off"
+#push-options "--fuel 2 --ifuel 1" //to unfold t_of
+#push-options "--query_stats"
+
+let hash_value_buf  = x:A.array U8.t { A.length x == 32}
+
+noeq
+type ha = {
+  acc: hash_value_buf;
+  ctr:R.ref U32.t
+}
+
+[@@__steel_reduce__;__reduce__]
+unfold
+let ha_perm (h:ha) =
+  A.varray h.acc `star` vptr h.ctr
+
+let ha_sl x = hp_of (ha_perm x)
+
+let ha_repr = A.contents U8.t 32 & U32.t
+
+let ha_sel x = sel_of (ha_perm x)
+
+let value_of x = fst x, U32.v (snd x)
 
 let initial_hash
-  = Seq.create 32 0uy
+  = Seq.create 32 0uy, 0
 
-let hash_value (s:Seq.seq U8.t { Seq.length s <= blake2_max_input_length })
+let hash_one_value (s:Seq.seq U8.t { Seq.length s <= blake2_max_input_length })
   : hash_value_t
-  = Blake.spec s 0 Seq.empty 32
+  = Blake.spec s 0 Seq.empty 32, 1
 
 noextract inline_for_extraction
 let xor_bytes (s1: Seq.seq U8.t)
@@ -32,11 +57,55 @@ let exor_bytes #l (s1 s2:elbytes l)
   : elbytes l
   = xor_bytes s1 s2
 
-let aggregate_hash_value (h0 h1: hash_value_t)
+let aggregate_hashes (h0 h1: hash_value_t)
   : hash_value_t
-  = xor_bytes h0 h1
+  = xor_bytes (fst h0) (fst h1),
+    snd h0 + snd h1
 
-let create_in (_:unit) = A.malloc 0uy 32ul
+let intro_ha_inv (#o:_) (s:ha)
+  : AT.SteelGhost unit o
+    (A.varray s.acc `star` R.vptr s.ctr)
+    (fun _ -> ha_inv s)
+    (requires fun _ -> True)
+    (ensures fun h0 _ h1 ->
+      hash_value_of s h1 ==
+        (A.asel s.acc h0,
+         U32.v (R.sel s.ctr h0)))
+  = AT.change_slprop_rel
+       (A.varray s.acc `star` R.vptr s.ctr)
+       (ha_inv s)
+       (fun x y -> x == y)
+       (fun m -> ())
+
+let elim_ha_inv #o (s:ha)
+  : AT.SteelGhost unit o
+    (ha_inv s)
+    (fun _ -> A.varray s.acc `star` R.vptr s.ctr)
+    (requires fun _ -> True)
+    (ensures fun h0 _ h1 ->
+      hash_value_of s h0 ==
+        (A.asel s.acc h1,
+         U32.v (R.sel s.ctr h1)))
+  = AT.change_slprop_rel
+       (ha_inv s)
+       (A.varray s.acc `star` R.vptr s.ctr)
+       (fun x y -> x == y)
+       (fun m -> ())
+
+let create (_:unit)
+  = let acc = A.malloc 0uy 32ul in
+    let ctr = R.malloc 0ul in
+    let ha = { acc; ctr } in
+    //TODO: this is annoying
+    AT.change_equal_slprop (A.varray acc `star` R.vptr ctr)
+                           (A.varray ha.acc `star` R.vptr ha.ctr);
+    intro_ha_inv ha;
+    AT.return ha
+
+let free (s:ha)
+  = elim_ha_inv s;
+    A.free s.acc;
+    R.free s.ctr
 
 let exor_bytes_pfx #l (s1 s2:elbytes l) (i:nat { i <= l })
   : elbytes l
@@ -44,14 +113,15 @@ let exor_bytes_pfx #l (s1 s2:elbytes l) (i:nat { i <= l })
       (exor_bytes #i (Seq.slice s1 0 i) (Seq.slice s2 0 i))
       (Seq.slice s1 i (Seq.length s1))
 
-let ehash_value_t = elbytes 32
 
-let upd_ehash_value (x:ehash_value_t) (i:nat{i < 32}) (v:U8.t)
-  : ehash_value_t
+let eraw_hash_t = elbytes 32
+
+let upd_ehash_value (x:eraw_hash_t) (i:nat{i < 32}) (v:U8.t)
+  : eraw_hash_t
   = Seq.upd x i v
 
 #push-options "--z3rlimit_factor 3"
-let extend_ehash_value (s1 s2:ehash_value_t) (i:nat { i < 32 })
+let extend_ehash_value (s1 s2:eraw_hash_t) (i:nat { i < 32 })
   : Lemma (upd_ehash_value
                      (exor_bytes_pfx s1 s2 i)
                      i
@@ -60,10 +130,11 @@ let extend_ehash_value (s1 s2:ehash_value_t) (i:nat { i < 32 })
   = ()
 #pop-options
 
-let hpts_to (x:hash_value_buf) (s:ehash_value_t) =
+
+let hpts_to (x:hash_value_buf) (s:eraw_hash_t) =
   A.varray_pts_to x s
 
-let read_hbuf (#s:ehash_value_t) (x:hash_value_buf) (i:U32.t{U32.v i < 32})
+let read_hbuf (#s:eraw_hash_t) (x:hash_value_buf) (i:U32.t{U32.v i < 32})
   : Steel U8.t
     (hpts_to x s)
     (fun _ -> hpts_to x s)
@@ -77,7 +148,7 @@ let read_hbuf (#s:ehash_value_t) (x:hash_value_buf) (i:U32.t{U32.v i < 32})
                            (hpts_to x s);
     AT.return v
 
-let write_hbuf (#s:ehash_value_t) (x:hash_value_buf) (i:U32.t{U32.v i < 32}) (v:U8.t)
+let write_hbuf (#s:eraw_hash_t) (x:hash_value_buf) (i:U32.t{U32.v i < 32}) (v:U8.t)
   : SteelT unit
     (hpts_to x s)
     (fun _ -> hpts_to x (upd_ehash_value s (U32.v i) v))
@@ -88,27 +159,27 @@ let write_hbuf (#s:ehash_value_t) (x:hash_value_buf) (i:U32.t{U32.v i < 32}) (v:
                            (hpts_to _ _)
 
 let intro_hpts_to (#o:_) (x:hash_value_buf)
-  : AT.SteelGhost ehash_value_t o
+  : AT.SteelGhost eraw_hash_t o
     (A.varray x)
     (fun v -> hpts_to x v)
     (requires fun _ -> True)
     (ensures fun h v _ ->
-      as_hash_value x h == Ghost.reveal v)
+      A.asel x h == Ghost.reveal v)
   = A.intro_varray_pts_to x
 
-let elim_hpts_to (#o:_) (#e:ehash_value_t) (x:hash_value_buf)
+let elim_hpts_to (#o:_) (#e:eraw_hash_t) (x:hash_value_buf)
   : AT.SteelGhost unit o
     (hpts_to x e)
     (fun _ -> A.varray x)
     (requires fun _ -> True)
     (ensures fun _ _ h ->
-      Ghost.reveal e == as_hash_value x h)
+      Ghost.reveal e == A.asel x h)
   = A.elim_varray_pts_to x e
 
 #push-options "--query_stats --fuel 0 --ifuel 0"
 let aggregate_hash_value_pts
-    (s1: ehash_value_t)
-    (s2: ehash_value_t)
+    (s1: eraw_hash_t)
+    (s2: eraw_hash_t)
     (b1: hash_value_buf)
     (b2: hash_value_buf)
   : SteelT unit
@@ -154,7 +225,14 @@ let aggregate_hash_value_pts
                            (hpts_to b1 _ `star` hpts_to b2 _);
     AT.return ()
 
-let aggregate_hash_value_buf (b1: hash_value_buf) (b2: hash_value_buf)
+let aggregate_raw_hashes (b1: hash_value_buf) (b2: hash_value_buf)
+  : Steel unit
+    (A.varray b1 `star` A.varray b2)
+    (fun _ -> A.varray b1 `star` A.varray b2)
+    (requires fun _ -> True)
+    (ensures fun h0 _ h1 ->
+      A.asel b2 h0 == A.asel b2 h1 /\
+      A.asel b1 h1 == xor_bytes (A.asel b1 h0) (A.asel b2 h0))
   = let _ = intro_hpts_to b1 in
     let _ = intro_hpts_to b2 in
     aggregate_hash_value_pts _ _ b1 b2;
@@ -162,23 +240,131 @@ let aggregate_hash_value_buf (b1: hash_value_buf) (b2: hash_value_buf)
     elim_hpts_to b2
 
 
-let add (s:hash_value_buf) (input:hashable_buffer) (l:U32.t)
-  = let tmp = A.malloc 0uy 32ul in
-    Blake.blake2b 32ul tmp l input;
-    aggregate_hash_value_buf s tmp;
-    A.free tmp;
-    let h1 = AT.get() in //Weird to need this
-    assert (A.asel s h1 == v_hash s h1);
-    AT.return ()
+inline_for_extraction
+let narrow_uint64_to_uint32 (x:U64.t { U64.(x <=^ 0xffffffffuL) })
+  : y:U32.t{U64.v x == U32.v y}
+  = Cast.uint64_to_uint32 x
 
-let get (s:state) (out:hash_value_buf)
-  : Steel unit
-    (A.varray s `star` A.varray out)
-    (fun _ -> A.varray s `star` A.varray out)
+let aggregate (b1 b2: ha)
+  = elim_ha_inv b1;
+    elim_ha_inv b2;
+    let ctr1 = R.read b1.ctr in
+    let ctr2 = R.read b2.ctr in
+    let ctr = U64.(
+      (Cast.uint32_to_uint64 ctr1)
+      +^
+      (Cast.uint32_to_uint64 ctr2)
+    )
+    in
+    if U64.(ctr >^ 0xffffffffuL)
+    then (
+      intro_ha_inv b1;
+      intro_ha_inv b2;
+      AT.return false
+    )
+    else (
+      aggregate_raw_hashes b1.acc b2.acc;
+      R.write b1.ctr (narrow_uint64_to_uint32 ctr);
+      intro_ha_inv b1;
+      intro_ha_inv b2;
+      AT.return true
+    )
+
+
+let compare (b1 b2:ha)
+  = AT.sladmit();
+    AT.return false
+
+let add (s:ha) (input:hashable_buffer) (l:U32.t)
+  = let acc = A.malloc 0uy 32ul in //TODO:would be nice to stack allocate this
+    let ctr = R.malloc 1ul in  //TODO:would be nice to stack allocate this
+    Blake.blake2b 32ul acc l input;
+    let ha' = { acc; ctr } in
+    AT.change_equal_slprop
+      (A.varray acc `star` R.vptr ctr)
+      (A.varray ha'.acc `star` R.vptr ha'.ctr);
+    intro_ha_inv ha';
+    let v = aggregate s ha' in
+    free ha';  //TODO:Then we wouldn't need this
+    AT.return v
+
+let ha_val (r:ha) (v:Ghost.erased hash_value_t)
+  : vprop
+  = A.varray_pts_to r.acc (fst v) `star`
+    AT.h_exists (fun (i:Ghost.erased U32.t) ->
+      pure (U32.v i == (snd v)) `star`
+      R.pts_to r.ctr Steel.FractionalPermission.full_perm i)
+
+
+let intro_ha_val #o (r:ha) (v:Ghost.erased hash_value_t)
+    : AT.SteelGhostT unit o
+      (A.varray_pts_to r.acc (fst v) `star`
+       AT.h_exists (fun (i:Ghost.erased U32.t) ->
+         pure (U32.v i == (snd v)) `star`
+         R.pts_to r.ctr Steel.FractionalPermission.full_perm i))
+      (fun _ -> ha_val r v)
+    = assert_spinoff
+         ((A.varray_pts_to r.acc (fst v) `star`
+            AT.h_exists (fun (i:Ghost.erased U32.t) ->
+              pure (U32.v i == (snd v)) `star`
+              R.pts_to r.ctr Steel.FractionalPermission.full_perm i)) ==
+          (ha_val r v));
+      AT.change_equal_slprop
+      (A.varray_pts_to r.acc (fst v) `star`
+       AT.h_exists (fun (i:Ghost.erased U32.t) ->
+         pure (U32.v i == (snd v)) `star`
+         R.pts_to r.ctr Steel.FractionalPermission.full_perm i))
+      (ha_val r v)
+
+let ha_val_of_ha_inv (#o:_) (s:ha)
+  : AT.SteelGhost (Ghost.erased hash_value_t) o
+    (ha_inv s)
+    (fun v -> ha_val s v)
     (requires fun _ -> True)
-    (ensures fun h0 _ h1 ->
-       v_hash s h0 == as_hash_value out h1 /\
-       v_hash s h1 == v_hash s h0)
-  = A.memcpy s out 32ul
+    (ensures fun h0 x _ ->
+       Ghost.reveal x == hash_value_of s h0)
+  = elim_ha_inv s;
+    let i = R.elim_vptr s.ctr _ in
+    let raw_hash = A.intro_varray_pts_to s.acc in
+    let v : Ghost.erased hash_value_t =
+        Ghost.hide (Ghost.reveal raw_hash, U32.v i)
+    in
+    AT.change_equal_slprop
+      (A.varray_pts_to s.acc raw_hash)
+      (A.varray_pts_to s.acc (fst v));
+    AT.intro_pure (U32.v i == snd v);
+    AT.intro_exists #(Ghost.erased U32.t) i
+      (fun i ->
+         pure (U32.v i == (snd v)) `star`
+         R.pts_to s.ctr Steel.FractionalPermission.full_perm i);
+    intro_ha_val s v;
+    v
 
-let free (s:state) = A.free s
+
+let elim_ha_val #o (r:ha) (v:Ghost.erased hash_value_t)
+    : AT.SteelGhostT unit o
+      (ha_val r v)
+      (fun _ -> A.varray_pts_to r.acc (fst v) `star`
+       AT.h_exists (fun (i:Ghost.erased U32.t) ->
+         pure (U32.v i == (snd v)) `star`
+         R.pts_to r.ctr Steel.FractionalPermission.full_perm i))
+    = assert_spinoff
+         ((A.varray_pts_to r.acc (fst v) `star`
+            AT.h_exists (fun (i:Ghost.erased U32.t) ->
+              pure (U32.v i == (snd v)) `star`
+              R.pts_to r.ctr Steel.FractionalPermission.full_perm i)) ==
+          (ha_val r v));
+      AT.change_equal_slprop
+      (ha_val r v)
+      (A.varray_pts_to r.acc (fst v) `star`
+       AT.h_exists (fun (i:Ghost.erased U32.t) ->
+         pure (U32.v i == (snd v)) `star`
+         R.pts_to r.ctr Steel.FractionalPermission.full_perm i))
+
+let ha_inv_of_ha_val #o #v (s:ha)
+  = elim_ha_val s v;
+    let i = AT.witness_exists () in
+    AT.elim_pure _;
+    A.elim_varray_pts_to s.acc _;
+    R.intro_vptr s.ctr _ _;
+    intro_ha_inv s
