steel/Veritas.Steel.HashAccumulator.fsti
@@ -2,7 +2,7 @@ module Veritas.Steel.HashAccumulator
 module U8 = FStar.UInt8
 module U32 = FStar.UInt32
 module A = Steel.Array
-
+open Steel.Memory
 open Steel.Effect.Common
 open Steel.Effect
 open Steel.Reference
@@ -16,92 +16,139 @@ noextract inline_for_extraction
 let hashable_bytes = s:Seq.seq U8.t { Seq.length s <= blake2_max_input_length }
 let hashable_buffer = b:A.array U8.t { A.length b <= blake2_max_input_length }
 
-let hash_value_t = Seq.lseq U8.t 32
+let hash_value_t = Seq.lseq U8.t 32 & nat
 
+val ha
+  : Type0
+
+val ha_sl (_:ha)
+  : slprop u#1
+
+val ha_repr
+  : Type0
+
+val ha_sel (x:ha)
+  : GTot (selector ha_repr (ha_sl x))
+
+[@@__steel_reduce__]
+noextract
+let ha_inv' (x:ha)
+  : GTot vprop'
+  = { hp = ha_sl x;
+      t = ha_repr;
+      sel = ha_sel x}
+
+unfold
+let ha_inv (r:ha)
+  : vprop
+  = VUnit (ha_inv' r)
+  
+[@@ __steel_reduce__]
+let repr_of (#p:vprop)
+            (r:ha)
+            (h:rmem p{FStar.Tactics.with_tactic selector_tactic
+                      (can_be_split p (ha_inv r) /\ True)})
+  : GTot ha_repr
+  = h (ha_inv r)
+
+val value_of (_:ha_repr)
+  : hash_value_t
+  
 val initial_hash
   : hash_value_t
 
-val hash_value (_:hashable_bytes)
+val hash_one_value (_:hashable_bytes)
   : hash_value_t
 
-val aggregate_hash_value (_ _: hash_value_t)
+val aggregate_hashes (_ _: hash_value_t)
   : hash_value_t
 
-let hash_value_buf = b:A.array U8.t{ A.length b == 32 }
-
-[@@ __steel_reduce__]
-let as_hash_value (#p:vprop) (r:hash_value_buf)
-    (h:rmem p{FStar.Tactics.with_tactic selector_tactic (can_be_split p (A.varray r) /\ True)})
-  = A.asel r h
-
-let state = hash_value_buf
-
-(* Can't introduce an abbreviation here ...
-   else v_hash fails *)
-// [@@__steel_reduce__;__reduce__]
-// unfold
-// let invariant (s: state) 
-//   : vprop
-//   = A.varray s
-
-let v_hash
-     (#p:vprop)
-     (t:state)
-     (h:rmem p{
-       FStar.Tactics.with_tactic
-         selector_tactic
-         (can_be_split p (A.varray t) /\ True)
-     })
+[@@__steel_reduce__]
+unfold
+let hash_value_of (#p:vprop)
+                  (r:ha)
+                  (h:rmem p{FStar.Tactics.with_tactic selector_tactic
+                            (can_be_split p (ha_inv r) /\ True)})
   : GTot hash_value_t
-  = A.asel t h
+  = value_of (repr_of r h)
+
 
 (*** THE MAIN INTERFACE ***)
 
 (** Create an instance of a hash accumulator in the heap *)
-val create_in (_:unit)
-  : Steel state
+val create (_:unit)
+  : Steel ha
     emp
-    (fun s -> A.varray s)
+    (fun s -> ha_inv s)
     (requires fun _ -> True)
     (ensures fun _ s h1 ->
-       v_hash s h1 == initial_hash)
-
-(** Combine two hash values held in b1 and b2 into b1 *)
-val aggregate_hash_value_buf (b1: hash_value_buf) (b2: hash_value_buf)
-  : Steel unit
-    (A.varray b1 `star` A.varray b2)
-    (fun _ -> A.varray b1 `star` A.varray b2)
-    (requires fun _ -> True)
-    (ensures fun h0 _ h1 ->
-      as_hash_value b2 h0 == as_hash_value b2 h1 /\
-      as_hash_value b1 h1 == aggregate_hash_value (as_hash_value b1 h0)
-                                                  (as_hash_value b2 h0))
-
-(** Hash the (input[0, l)) into the hash accumulate s *)
-val add (s:state) (input:hashable_buffer) (l:U32.t)
-  : Steel unit
-    (A.varray s `star` A.varray input)
-    (fun _ -> A.varray s `star` A.varray input)    
-    (requires fun h0 ->
-      U32.v l <= A.length input)
-    (ensures fun h0 _ h1 ->
-      U32.v l <= A.length input /\    
-      v_hash s h1 ==
-      aggregate_hash_value (v_hash s h0)
-                           (hash_value (Seq.slice (A.asel input h0) 0 (U32.v l))))
-
-(** Read the current value of the hash into out *)
-val get (s:state) (out:hash_value_buf)
-  : Steel unit
-    (A.varray s `star` A.varray out)
-    (fun _ -> A.varray s `star` A.varray out)
-    (requires fun h0 -> True)
-    (ensures fun h0 r h1 ->
-      v_hash s h0 == as_hash_value out h1 /\
-      v_hash s h1 == v_hash s h0)
+       hash_value_of s h1 == initial_hash)
 
 (** Free the hash accumulator *)
-val free (s:state)
+val free (s:ha)
   : SteelT unit
-    (A.varray s)
+    (ha_inv s)
     (fun _ -> emp)
+
+//TODO: can't inline this if in the ensures of aggregate
+let maybe_aggregate_hashes (b:bool) (h0 h1: hash_value_t) =
+  if b then aggregate_hashes h0 h1
+  else h0
+
+val aggregate (b1 b2: ha)
+  : Steel bool
+    (ha_inv b1 `star` ha_inv b2)
+    (fun _ -> ha_inv b1 `star` ha_inv b2)
+    (requires fun _ -> True)
+    (ensures fun h0 success h1 ->
+      hash_value_of b2 h0 == hash_value_of b2 h1 /\
+      hash_value_of b1 h1 ==
+        maybe_aggregate_hashes success
+          (hash_value_of b1 h0)
+          (hash_value_of b2 h0))
+
+val compare (b1 b2:ha)
+  : Steel bool
+    (ha_inv b1 `star` ha_inv b2)
+    (fun _ -> ha_inv b1 `star` ha_inv b2)
+    (requires fun _ -> True)
+    (ensures fun h0 success h1 ->
+      hash_value_of b1 h0 == hash_value_of b1 h1 /\
+      hash_value_of b2 h0 == hash_value_of b2 h1 /\
+      success = (hash_value_of b1 h1 = hash_value_of b2 h1))
+  
+(** Hash the (input[0, l)) into the hash accumulate s *)
+val add (s:ha) (input:hashable_buffer) (l:U32.t)
+  : Steel bool
+    (ha_inv s `star` A.varray input)
+    (fun _ -> ha_inv s `star` A.varray input)    
+    (requires fun h0 ->
+      U32.v l <= A.length input)
+    (ensures fun h0 success h1 ->
+      U32.v l <= A.length input /\    
+      hash_value_of s h1 ==
+        maybe_aggregate_hashes success
+          (hash_value_of s h0)
+          (hash_one_value (Seq.slice (A.asel input h0) 0 (U32.v l))))
+
+(* An indexed variant of ha_inv *)
+module AT = Steel.Effect.Atomic
+
+val ha_val (r:ha) (v:Ghost.erased hash_value_t)
+  : vprop
+
+val ha_val_of_ha_inv (#o:_) (s:ha)
+  : AT.SteelGhost (Ghost.erased hash_value_t) o
+    (ha_inv s)
+    (fun v -> ha_val s v)
+    (requires fun _ -> True)
+    (ensures fun h0 x _ -> 
+       Ghost.reveal x == hash_value_of s h0)
+
+val ha_inv_of_ha_val (#o:_) (#v:Ghost.erased hash_value_t) (s:ha)
+  : AT.SteelGhost unit o
+    (ha_val s v)
+    (fun _ -> ha_inv s)
+    (requires fun _ -> True)
+    (ensures fun _ _ h1 ->
+       hash_value_of s h1 == Ghost.reveal v)
